Initial delete

Treap.dfy
@@ -3,26 +3,192 @@ include "TreapNode.dfy"
 class Treap {
   var root: TreapNode?
   var prioritySet: set<int> //Keeps track of what priority was used.
+  ghost var repr: set<object> //Keeps track of what priority was used.
 
-  constructor () {
+  constructor ()
+    ensures Valid()
+  {
     this.root := null;
+    repr := {this};
   }
 
   ghost predicate Valid()
     reads this, root, if root != null then root.repr else {}
   {
-    root != null ==> root.Valid()
+    && root != null ==> (root.Valid() && root in repr)
   }
 
 
   method Build(values: array<int>) {}
   method Insert(value: int) {}
-  method Delete(value: int) {
+
+  // method Delete(value: int)
+  //   requires Valid()
+  //   modifies this
+  //   ensures Valid()
+  // {
+  //   if (root != null) {
+  //     var parent, node := SearchParentNode(root, value);
+  //     if (node != null) {
+  //       DeleteNode(parent, node);
+  //     }
+  //   }
+  // }
+
+  // method DeleteNode(parent: TreapNode?, node: TreapNode)
+  //   requires Valid()
+  //   requires node.Valid()
+  //   requires parent != null ==> parent.Valid()
+  //   requires parent != null ==> node == parent.left || node == parent.right
+  //   modifies this, parent, node
+  //   ensures parent != null ==> parent.Valid()
+  //   ensures Valid()
+  // {
+  //   if(node.IsLeaf()) {
+  //     if(parent != null) {
+  //       if(parent.left == node) {
+  //         parent.repr := parent.repr - parent.left.repr;
+  //         parent.left := null;
+  //         return;
+  //       }
+  //       // if(parent.right == node) {
+  //       //   parent.right := null;
+  //       //   return;
+  //       // }
+  //     }
+  //   }
+  // }
+
+  method Delete(value: int)
+    modifies this, root, if root != null then root.repr else {}
+    requires Valid()
+    ensures Valid()
+  {
+    if (root != null) {
+      this.root := DeleteNode(root, value);
+      if (root != null) {
+        repr := repr + root.repr;
+      }
+    }
   }
+
+  method editroot()
+    modifies this, root, if root != null then root.repr else {}
+    requires Valid()
+    ensures Valid()
+  {
+    if(root != null) {
+      root := addleft(root);
+      repr := repr + root.repr;
+    }
+  }
+
+  method addleft(node: TreapNode)
+    returns (newNode:TreapNode)
+    modifies node.repr
+    requires node.Valid()
+    ensures newNode.Valid()
+  {
+    newNode := node;
+    assert newNode.Valid();
+    if (newNode.left == null){
+      newNode.left := new TreapNode(1,2);
+      newNode.repr := newNode.repr + newNode.left.repr;
+    }
+  }
+
+  method DeleteNode(currRoot: TreapNode, value: int)
+    returns (newNode: TreapNode?)
+    modifies currRoot.repr
+    requires currRoot.Valid()
+    ensures newNode != null ==> newNode.Valid()
+    ensures newNode != null ==> fresh(newNode.repr - old(currRoot.repr))
+    decreases currRoot.repr
+  {
+    newNode := currRoot;
+    assert newNode.Valid();
+    if (newNode.left != null && value < newNode.key) {
+      assert newNode.left.Valid();
+      var newLeft := DeleteNode(newNode.left, value);
+      newNode.left :=  newLeft;
+      if(newLeft != null) {
+        newNode.repr := newNode.repr + newNode.left.repr;
+      }
+    } else if (newNode.right != null && value > newNode.key){
+      var newRight := DeleteNode(newNode.right, value);
+      newNode.right := newRight;
+      if(newRight != null) {
+        newNode.repr := newNode.repr + newNode.right.repr;
+      }
+    } else if (newNode.key == value) {
+      // Delete
+      if (newNode.IsLeaf()) {
+        newNode := null;
+      } else if (newNode.left == null) {
+        newNode := newNode.right;
+      } else if (newNode.right == null){
+        newNode := newNode.left;
+      } else {
+        // Check priority and rotate accordingly
+        if (newNode.right.priority >= newNode.left.priority) {
+          newNode := RotateLeft(newNode);
+          var newNodeLeft := DeleteNode(newNode.left, value);
+          newNode.left := newNodeLeft;
+          if(newNodeLeft != null) {
+            newNode.repr := newNode.repr + newNodeLeft.repr;
+          }
+        } else {
+          newNode := RotateRight(newNode);
+          var newNodeRight := DeleteNode(newNode.right, value);
+          newNode.right := newNodeRight;
+          if(newNodeRight != null) {
+            newNode.repr := newNode.repr + newNodeRight.repr;
+          }
+        }
+      }
+    }
+  }
+
+  // method BubbleDown(currParent: TreapNode?, node: TreapNode)
+  //   requires Valid()
+  //   requires node.Valid()
+  //   requires currParent != null ==> currParent.Valid()
+  //   requires currParent != null ==> (currParent.left == node || currParent.right == node)
+  //   modifies this, currParent, node, node.repr
+  //   ensures currParent != null && currParent.left == node ==> currParent.repr == old(currParent.repr)
+  //   ensures Valid()
+  //   {
+  //     // node has children
+  //     if(!node.IsLeaf()) {
+  //       var left := node.left;
+  //       var right := node.right;
+  //       var newRoot := node;
+  //       if(left != null && right != null) {
+  //         // rotate right if left priority is bigger
+  //         if(left.priority > right.priority) {
+  //           newRoot := RotateRight(node);
+  //         } else {
+  //           newRoot := RotateLeft(node);
+  //         }
+  //       } else if (right != null) {
+  //           newRoot := RotateLeft(node);
+  //       } else if (left != null) {
+  //           newRoot := RotateRight(node);
+  //       }
+  //       // if(currParent != null) {
+  //       //   if(currParent.left == node) {
+  //       //     currParent.left := newRoot;
+  //       //   }
+  //       // }
+  //     }
+  //   }
 
   // Initial search entry point
   method Search(value: int) returns (node: TreapNode?)
-    requires Valid()
+    requires Valid() // Tree is valid before search
+    ensures Valid() // Tress is valid after search
+    ensures if node != null then node.key == value else true // Return node has correct value
+    ensures if node != null then node.Valid() else true // Return node is valid
   {
     if(root == null){
       return null;
@@ -35,7 +201,8 @@ class Treap {
   method SearchNode(currRoot: TreapNode, value: int)
     returns (node: TreapNode?)
     requires currRoot.Valid()
-    ensures if node != null then node.key == value else true
+    ensures node != null ==> node.key == value
+    ensures node != null ==> node.Valid()
     decreases currRoot.repr
   {
     if (currRoot.key == value) {
@@ -52,7 +219,54 @@ class Treap {
     return null;
   }
 
-  method RotateLeft(node: TreapNode)
+  // Recursive search with parent node returned too, useful for delete
+  method ParentNode(currRoot: TreapNode, targetNode: TreapNode)
+    returns (parent: TreapNode?)
+    requires Valid()
+    requires currRoot.Valid()
+    requires targetNode.Valid()
+    ensures parent != null ==> parent.Valid()
+    ensures parent != null ==> (parent.left == targetNode || parent.right == targetNode)
+    ensures Valid()
+    decreases currRoot.repr
+  {
+    if (currRoot == targetNode) {
+      return null;
+    }
+    if (currRoot.left == targetNode || currRoot.right == targetNode) {
+      return currRoot;
+    }
+    if (targetNode.key > currRoot.key && currRoot.right != null) {
+      parent := ParentNode(currRoot.right, targetNode);
+      return parent;
+    }
+    if (targetNode.key <= currRoot.key && currRoot.left!= null) {
+      parent := ParentNode(currRoot.left, targetNode);
+      return parent;
+    }
+    return null;
+  }
+
+  // ghost method DeleteRepr(currRoot: TreapNode, node: TreapNode)
+  //   requires Valid()
+  //   requires currRoot.Valid()
+  //   modifies currRoot.repr
+  //   // ensures Valid()
+  //   decreases currRoot.repr
+  // {
+  //   if(node in currRoot.repr) {
+  //     if(currRoot.left != null && node in currRoot.left.repr) {
+  //       DeleteRepr(currRoot.left, node);
+  //     }
+  //     if(currRoot.right != null && node in currRoot.right.repr) {
+  //       DeleteRepr(currRoot.right, node);
+  //     }
+  //     currRoot.repr := currRoot.repr - {node};
+  //   }
+  // }
+
+
+  static method RotateLeft(node: TreapNode)
     returns (newNode: TreapNode)
     requires node.right != null
     requires node.Valid()
@@ -72,20 +286,21 @@ class Treap {
     node.right:= tempNode;
     if(tempNode != null) {
       // need to add repr of tempNode into node to maintain validity
-      node.repr := node.repr + tempNode.repr + {tempNode};
+      assert tempNode.Valid();
+      node.repr := node.repr + tempNode.repr;
     }
     newNode.repr := newNode.repr + node.repr;
-    return newNode;
   }
 
-  method RotateRight(node: TreapNode)
+  static method RotateRight(node: TreapNode)
     returns (newNode: TreapNode)
-    requires node.left != null
     requires node.Valid()
+    requires node.left != null
     modifies node.repr
     ensures newNode.Valid()
+    ensures old(node.repr) == newNode.repr // No change in reachability
     ensures newNode == old(node.left)
-    ensures newNode.left== old(newNode.left)
+    ensures newNode.left == old(newNode.left)
     ensures newNode.right == node
     ensures node.left == old(node.left.right)
     ensures node.right== old(node.right)
@@ -97,10 +312,10 @@ class Treap {
     node.left := tempNode;
     if(tempNode != null) {
       // need to add repr of tempNode into node to maintain validity
-      node.repr := node.repr + tempNode.repr + {tempNode};
+      assert tempNode.Valid();
+      node.repr := node.repr + tempNode.repr;
     }
     newNode.repr := newNode.repr + node.repr;
-    return newNode;
   }
 
   // To allow for different implementation of RNG
@@ -108,11 +323,36 @@ class Treap {
   method RandomNumberGenerator() returns (priority: int) {
     return -1;
   }
+
+  method test()
+    modifies this
+    requires Valid()
+    ensures Valid()
+  {
+    var root := new TreapNode(5,10);
+    var left := new TreapNode(2,4);
+    var right := new TreapNode(7,5);
+    root.left := left;
+    root.right := right;
+    root.repr := {root, left, right};
+    assert left.Valid();
+    assert right.Valid();
+    assert root.Valid();
+    this.root := root;
+    // Delete(5);
+  }
+
 }
 
 // Used for testing
 method Main() {
   var treap := new Treap();
-  var result := treap.RandomNumberGenerator();
+  treap.test();
+
+  var result := treap.Search(10);
+  var result2 := treap.Search(5);
+  treap.Delete(5);
   print (result);
+  print ("\n");
+  print (result2);
 }
